6/2*3 = 9
    PEMDAS says 1

https://www.huffingtonpost.ca/entry/math-problem-twitter-bedmas-pemdas_ca_5d420367e4b0acb57fc6b0fd

    (2/3) / (3/7) =
        {reciprocal of 2nd fraction}
    (2/3) * (7/3) = 
    (2*7)/(3*3) = 14/9

Now try with a zero in the numerator:

    (2/3) / (0/7) =
        {reciprocal of 2nd fraction}
    (2/3) * (7/0) =
    (2*7)/(3*0) = 14/0 = BOOM

Now try with a zero in the denominator:

    (2/3) / (3/0) =
        {reciprocal of 2nd fraction}
    (2/3) * (0/3) =
    (2*0)/(3*3) = 0/3

How is this rule consistent with PEMDAS?

etc.

60 / 5(7-5) = 24

    Following PEMDAS
        60 / 5(2) = 
        60 / 10 =
        6
